lots of bug fixes. malloc works now.

src/CancelTacIL.v
@@ -4,6 +4,7 @@ Require MirrorShard.ExprUnify.
 Require Import MirrorShard.Expr.
 Require Import MirrorShard.Reflection.
 Require Import MirrorShard.Provers.
+Require Import MirrorShard.SepExprTac.
 Require Import ILEnv SepIL TacPackIL.
 
 Set Implicit Arguments.
@@ -15,110 +16,50 @@ Module CANCEL_TAC :=
                                     ExprUnify.UNIFIER
                                     UNF.
 
+Module SEP_TAC := MirrorShard.SepExprTac.Make SepIL.ST SepIL.SEP.
+
 Section canceller.
   Variable ts : list Expr.type.
   Let types := Env.repr BedrockCoreEnv.core ts.
+  
+  Definition nsubstInEnv (not : Prop -> Prop) (types : list type) (funcs : functions types)
+    (meta_base var_env : env types) (sub : ExprUnify.UNIFIER.Subst types) :=
+    fix substInEnv (from : nat) (vals : env types) (ret : env types -> Prop)
+    {struct vals} : Prop :=
+    match vals with
+      | nil => ret nil
+      | val :: vals0 =>
+        match ExprUnify.UNIFIER.Subst_lookup from sub with
+          | Some v =>
+            match ExprTac.nexprD not _ funcs meta_base var_env v (projT1 val) with
+              | Some v' =>
+                projT2 val = v' /\
+                substInEnv (S from) vals0
+                (fun e : env types =>
+                  ret (existT (tvarD types) (projT1 val) v' :: e))
+              | None => CANCEL_TAC.ExistsSubstNone (projT1 val) v
+            end
+          | None =>
+            substInEnv (S from) vals0 (fun e : env types => ret (val :: e))
+        end
+    end.
 
+  Theorem nsubstInEnv_substInEnv : nsubstInEnv not = CANCEL_TAC.substInEnv.
+  Proof. reflexivity. Qed.
 
-
-(*
-  Theorem ApplyCancelSep_with_eq1 :
-    forall (funcs : functions types) (preds : SEP.predicates types)
-      (algos : TacPackIL.ILAlgoTypes.AllAlgos types)
-      (algosC : @TacPackIL.ILAlgoTypes.AllAlgos_correct types funcs preds algos)
-      (uvars : env types) (lhs rhs : SEP.sexpr types)
-      (hyps : exprs types)
-      (cr : CANCEL_LOOP.cancelResult types),
-      AllProvable funcs uvars nil hyps ->
-      (let bound := 10 in
-       let hints :=
-         match TacPackIL.ILAlgoTypes.Hints algos with
-           | None => {| UNF.Forward := nil ; UNF.Backward := nil |}
-           | Some x => x
-         end
-       in
-       let prover :=
-         match TacPackIL.ILAlgoTypes.Prover algos with
-           | None => Provers.trivialProver types
-           | Some x => x
-         end
-       in
-       let '(x,y) :=
-         CANCEL_LOOP.cancel (SEP.typeof_preds preds) prover (UNF.Forward hints) (UNF.Backward hints)
-         bound hyps (typeof_env uvars) nil lhs rhs in
-       (x, SEP.WellTyped_sexpr (typeof_funcs funcs) (SEP.typeof_preds preds) (typeof_env uvars) nil rhs && y) = (cr, true)) ->
-      CANCEL_LOOP.cancelResultD funcs preds uvars nil 0 cr ->
-      SEP.himp funcs preds uvars nil lhs rhs.
-  Proof.
-  Admitted.
-
-  Theorem ApplyCancelSep_with_eq2 :
-    forall (funcs : functions types) (preds : SEP.predicates types)
-      (algos : TacPackIL.ILAlgoTypes.AllAlgos types)
-      (algosC : @TacPackIL.ILAlgoTypes.AllAlgos_correct types funcs preds algos)
-      (uvars : env types) (lhs rhs : SEP.sexpr types)
-      (hyps : exprs types),
-      AllProvable funcs uvars nil hyps ->
-      (let bound := 10 in
-       let hints :=
-         match TacPackIL.ILAlgoTypes.Hints algos with
-           | None => {| UNF.Forward := nil ; UNF.Backward := nil |}
-           | Some x => x
-         end
-       in
-       let prover :=
-         match TacPackIL.ILAlgoTypes.Prover algos with
-           | None => Provers.trivialProver types
-           | Some x => x
-         end
-       in
-       let '(x,y) :=
-         CANCEL_LOOP.cancel (SEP.typeof_preds preds) prover (UNF.Forward hints) (UNF.Backward hints)
-         bound hyps (typeof_env uvars) nil lhs rhs in
-       if SEP.WellTyped_sexpr (typeof_funcs funcs) (SEP.typeof_preds preds) (typeof_env uvars) nil rhs && y then
-         CANCEL_LOOP.cancelResultD funcs preds uvars nil 0 x
-       else
-         SEP.himp funcs preds uvars nil lhs rhs) ->      
-      SEP.himp funcs preds uvars nil lhs rhs.
-  Proof.
-  Admitted.
-*)
-
-  Definition nsexprD (emp : hprop) (star : hprop -> hprop -> hprop) (ex : forall T : Type, (T -> hprop) -> hprop) (inj : Prop -> hprop) :=
-    fun (types : list Expr.type) (funcs : Expr.functions types)
-      (sfuncs : SEP.predicates types) =>
-      fix sexprD (meta_env var_env : Expr.env types) (s : SEP.sexpr types)
-      {struct s} : hprop :=
-      match s with
-        | SEP.Emp => emp
-        | SEP.Inj p =>
-          match Expr.exprD funcs meta_env var_env p Expr.tvProp with
-            | Some p0 => inj p0
-            | None => inj (SepExpr.BadInj p)
-          end
-        | SEP.Star l r =>
-          star (sexprD meta_env var_env l) (sexprD meta_env var_env r)
-        | SEP.Exists t b =>
-          ex _
-          (fun x : Expr.tvarD types t =>
-            sexprD meta_env (@existT _ (Expr.tvarD types) t x :: var_env) b)
-        | SEP.Func f b =>
-          match nth_error sfuncs f with
-            | Some f' =>
-              match
-                Expr.applyD (Expr.exprD funcs meta_env var_env) 
-                (SEP.SDomain f') b hprop (SEP.SDenotation f')
-                with
-                | Some p => p
-                | None => inj (SepExpr.BadPredApply f b var_env)
-              end
-            | None => inj (SepExpr.BadPred f)
-          end
-        | SEP.Const p => p
-      end.
+  Definition nexistsSubst (not : Prop -> Prop) := 
+    fun (types : list type) (funcs : functions types) (var_env : env types)
+      (sub : ExprUnify.UNIFIER.Subst types) (from : nat)
+      (vals : list {t : tvar & option (tvarD types t)}) 
+      (ret : env types -> Prop) =>
+      CANCEL_TAC.existsMaybe vals
+      (fun e : env types => nsubstInEnv not funcs e var_env sub from e ret).
+  
+  Theorem nexistsSubst_existsSubst : nexistsSubst not = CANCEL_TAC.existsSubst.
+  Proof. reflexivity. Qed.
 
   Definition cancel (himp : hprop -> hprop -> Prop) (emp : hprop) (star : hprop -> hprop -> hprop) 
-    (ex : forall T : Type, (T -> hprop) -> hprop) (inj : Prop -> hprop)
+    (ex : forall T : Type, (T -> hprop) -> hprop) (inj : Prop -> hprop) (not : Prop -> Prop)
     (ts : list Expr.type)
     (funcs : Expr.functions (Env.repr ILEnv.BedrockCoreEnv.core ts))
     (preds : SEP.predicates (Env.repr ILEnv.BedrockCoreEnv.core ts))
@@ -146,8 +87,8 @@ Section canceller.
     if SEP.WellTyped_sexpr tfuncs tpreds (typeof_env uvars) nil rhs then
       match CANCEL_TAC.canceller tpreds (TacPackIL.UNF.Forward hints) (TacPackIL.UNF.Backward hints) prover (typeof_env uvars) hyps lhs rhs with
         | None => 
-          himp (nsexprD emp star ex inj funcs preds uvars nil lhs)
-               (nsexprD emp star ex inj funcs preds uvars nil rhs)
+          himp (SEP_TAC.nsexprD not emp star ex inj types funcs preds uvars nil lhs)
+               (SEP_TAC.nsexprD not emp star ex inj types funcs preds uvars nil rhs)
         | Some {| CANCEL_TAC.AllExt := new_vars
                 ; CANCEL_TAC.ExExt := new_uvars
                 ; CANCEL_TAC.Lhs := lhs'
@@ -155,8 +96,8 @@ Section canceller.
                 ; CANCEL_TAC.Subst := subst |} =>
           forallEach new_vars (fun nvs : env types =>
              let var_env := nvs in
-             AllProvable_impl funcs uvars var_env
-               (CANCEL_TAC.existsSubst funcs var_env subst 0
+             ExprTac.nAllProvable_impl not _ funcs uvars var_env
+               (nexistsSubst not funcs var_env subst 0
                  (map
                    (fun x : sigT (tvarD types) =>
                        existT (fun t : tvar => option (tvarD types t))
@@ -166,15 +107,15 @@ Section canceller.
                        existT (fun t : tvar => option (tvarD types t)) x None)
                       new_uvars)
                    (fun meta_env0 : env types =>
-                    AllProvable_and funcs meta_env0 var_env
+                    ExprTac.nAllProvable_and not _ funcs meta_env0 var_env
                       (himp
-                         (nsexprD emp star ex inj funcs preds meta_env0 var_env
+                         (SEP_TAC.nsexprD not emp star ex inj types funcs preds meta_env0 var_env
                             (SH.sheapD
                                {|
                                SH.impures := SH.impures lhs';
                                SH.pures := nil;
                                SH.other := SH.other lhs' |}))
-                         (nsexprD emp star ex inj funcs preds meta_env0 var_env
+                         (SEP_TAC.nsexprD not emp star ex inj types funcs preds meta_env0 var_env
                             (SH.sheapD
                                {|
                                SH.impures := SH.impures rhs';
@@ -184,8 +125,8 @@ Section canceller.
 
       end
     else
-      himp (nsexprD emp star ex inj funcs preds uvars nil lhs)
-           (nsexprD emp star ex inj funcs preds uvars nil rhs).
+      himp (SEP_TAC.nsexprD not emp star ex inj types funcs preds uvars nil lhs)
+           (SEP_TAC.nsexprD not emp star ex inj types funcs preds uvars nil rhs).
       
 
   Theorem ApplyCancelSep_slice : forall (ts : list Expr.type)
@@ -198,7 +139,7 @@ Section canceller.
         (lhs rhs : SEP.sexpr (Env.repr ILEnv.BedrockCoreEnv.core ts))
         (hyps : Expr.exprs (Env.repr ILEnv.BedrockCoreEnv.core ts)),
         Expr.AllProvable funcs uvars nil hyps ->
-        (cancel himp emp star ex inj funcs preds algos uvars lhs rhs hyps) ->
+        (cancel himp emp star ex inj not funcs preds algos uvars lhs rhs hyps) ->
 (*           
          let '(x, y) :=
            CancelTacIL.CANCEL_LOOP.cancel (SEP.typeof_preds preds)
@@ -236,7 +177,16 @@ Section canceller.
       { destruct X. destruct (ILAlgoTypes.Hints algos); eauto using UNF.BackwardOk.
         simpl. constructor. }
       { destruct X. destruct (ILAlgoTypes.Prover algos); eauto using trivialProver_correct. }
-      { eapply typeof_funcs_WellTyped_funcs. } }
+      { eapply typeof_funcs_WellTyped_funcs. } 
+      { rewrite nexistsSubst_existsSubst in *. 
+        destruct c. apply forallEach_sem. intros.
+        eapply forallEach_sem in H2; eauto.
+        rewrite ExprTac.nAllProvable_impl_AllProvable_impl in H2.
+        apply AllProvable_impl_sem; intros.
+        apply AllProvable_impl_sem in H2; eauto.
+        eapply CANCEL_TAC.existsSubst_sem in H2. eapply existsEach_sem in H2. destruct H2; intuition.
+        eapply CANCEL_TAC.existsSubst_sem. eapply existsEach_sem. exists x. intuition.
+        rewrite ExprTac.nAllProvable_and_AllProvable_and in H8. auto. } }
     { apply H2. }
   Qed.
 
